Test/ast/function.dfy
@@ -2,9 +2,9 @@
 // RUN: ! %baredafny run --use-basename-for-filename "%s" >> "%t"
 // RUN: %diff "%s.expect" "%t"
 
-function method Foo(): int
-function method {:axiom} Bar(): int
-function method {:extern} Baz(): int
+function method Foo(): int ensures false; ensures false;
+function method {:axiom} Bar(): int ensures false;
+function method {:extern} Baz(): int ensures false;
 
 trait Far {
   function method Foo(): int
