Test/ast/method.dfy
@@ -2,5 +2,5 @@
 // RUN: ! %baredafny run --use-basename-for-filename "%s" >> "%t"
 // RUN: %diff "%s.expect" "%t"
 
-method Foo()
-method {:axiom} Bar()
+method Foo() ensures false; ensures false;
+method {:axiom} Bar() ensures false;
