Test/traits/TraitCompileErrors.dfy
@@ -4,13 +4,13 @@
 module StaticMembers {
   trait Tr {
     // the following static members must also be given bodies, but that's checked by the compiler
-    static function method Func(): int
-    static method Method()
-    static twostate function TwoF(): int
-    static twostate lemma TwoL()
+    static function method Func(): int ensures false
+    static method Method() ensures false
+    static twostate function TwoF(): int ensures false
+    static twostate lemma TwoL() ensures false
     static least predicate P()
     static greatest predicate Q()
-    static least lemma IL()
-    static greatest lemma CL()
+    static least lemma IL() ensures false
+    static greatest lemma CL() ensures false
   }
 }
